In the context of given example from the book, it's same to equalizer. (Of course it's mostly not in outside of the context. Check out [wikipedia](https://en.wikipedia.org/wiki/Coequalizer))

I'll use the same example the book used explaining equalizer.


## equalizer

$ACx=BCx$  
$\rightarrow \left( A-B\right) Cx=0$  
$\rightarrow \left( \left( 1\enspace 2\right) -\left( -1\enspace 1\right) \right) C=0$  
$\rightarrow \left( 2\enspace 1\right) C=0$  
$\rightarrow C=\begin{pmatrix}1 \\ -2\end{pmatrix}$  

## coequalizer

$CA\begin{pmatrix}x \\y\end{pmatrix}=CB\begin{pmatrix}x \\ y\end{pmatrix}$  
$\rightarrow CA-CB=0$  
$\rightarrow C\left( A-B\right) =0$  
$\rightarrow C\left( 2\enspace 1\right) =0$  
$\rightarrow C=\begin{pmatrix}1 \\-2\end{pmatrix}$  